Hashmap/DHashMap/Lemmas.lean
@@ -9,40 +9,60 @@ set_option autoImplicit false
 
 universe u v
 
-variable {α : Type u} {β : α → Type v}
+variable {α : Type u} {β : α → Type v} [BEq α] [Hashable α] [EquivBEq α] [LawfulHashable α]
 
 namespace MyLean.DHashMap
 
 namespace Raw₀
 
-theorem findEntry?ₘ_insert [BEq α] [EquivBEq α] [Hashable α] [LawfulHashable α]
-    (m : Raw₀ α β) (h : m.1.WF) (a k : α) (b : β a) :
-    findEntry?ₘ (m.insertₘ a b) k = bif a == k then some ⟨a, b⟩ else findEntry?ₘ m k := by
+variable (m : Raw₀ α β) (h : m.1.WF)
+
+/-! # Lemmas about model implementations -/
+
+theorem findEntry?ₘ_insertₘ (a k : α) (b : β a) :
+    (m.insertₘ a b).findEntry?ₘ k = bif a == k then some ⟨a, b⟩ else m.findEntry?ₘ k := by
   rw [findEntry?ₘ_eq_findEntry? _ (wfImp_insertₘ _ h.out _ _), findEntry?ₘ_eq_findEntry? _ h.out,
     List.findEntry?_of_perm (wfImp_insertₘ _ h.out _ _).distinct (toListModel_insertₘ _ h.out _ _),
     List.findEntry?_insertEntry]
 
-theorem findEntry?_insert [BEq α] [EquivBEq α] [Hashable α] [LawfulHashable α]
-    (m : Raw₀ α β) (h : m.1.WF) (a k : α) (b : β a) :
+theorem containsₘ_eq_isSome_findEntry?ₘ {a : α} : m.containsₘ a = (m.findEntry?ₘ a).isSome := by
+  rw [findEntry?ₘ_eq_findEntry? _ h.out, containsₘ_eq_containsKey h.out, List.containsKey_eq_isSome_findEntry?]
+
+/-! # Lemmas about actual implementations -/
+
+theorem findEntry?_insert (a k : α) (b : β a) :
     (m.insert a b).1.findEntry? k = bif a == k then some ⟨a, b⟩ else m.findEntry? k := by
-  rw [findEntry?_eq_findEntry?ₘ, insert_eq_insertₘ, findEntry?_eq_findEntry?ₘ, findEntry?ₘ_insert _ h]
+  rw [findEntry?_eq_findEntry?ₘ, insert_eq_insertₘ, findEntry?_eq_findEntry?ₘ, findEntry?ₘ_insertₘ _ h]
+
+theorem contains_eq_isSome_findEntry? {a : α} : m.contains a = (m.findEntry? a).isSome := by
+  rw [findEntry?_eq_findEntry?ₘ, contains_eq_containsₘ, containsₘ_eq_isSome_findEntry?ₘ _ h]
 
 end Raw₀
 
 namespace Raw
 
-theorem findEntry?_insert [BEq α] [EquivBEq α] [Hashable α] [LawfulHashable α]
-    (m : Raw α β) (h : m.WF) {a k : α} {b : β a} :
+variable (m : Raw α β) (h : m.WF)
+
+theorem findEntry?_insert {a k : α} {b : β a} :
     (m.insert a b).findEntry? k = bif a == k then some ⟨a, b⟩ else m.findEntry? k := by
-  rw [insert_eq h, findEntry?_eq, findEntry?_eq, Raw₀.findEntry?_insert]
-  · exact h
-  · exact h
-  · exact h.insert₀
+  rw [insert_eq h, findEntry?_eq h, findEntry?_eq h.insert₀, Raw₀.findEntry?_insert ⟨m, _⟩ h]
+
+theorem contains_eq_isSome_findEntry? {a : α} : m.contains a = (m.findEntry? a).isSome := by
+  rw [contains_eq h, findEntry?_eq h, Raw₀.contains_eq_isSome_findEntry? ⟨m, _⟩ h]
 
 end Raw
 
-theorem findEntry?_insert [BEq α] [EquivBEq α] [Hashable α] [LawfulHashable α] (m : DHashMap α β) (a k : α) (b : β a) :
+section
+
+variable (m : DHashMap α β)
+
+theorem findEntry?_insert (a k : α) (b : β a) :
     (m.insert a b).findEntry? k = bif a == k then some ⟨a, b⟩ else m.findEntry? k :=
   Raw₀.findEntry?_insert ⟨m.1, _⟩ m.2 a k b
+
+theorem contains_eq_isSome_findEntry? {a : α} : m.contains a = (m.findEntry? a).isSome :=
+  Raw₀.contains_eq_isSome_findEntry? ⟨m.1, _⟩ m.2
+
+end
 
 end MyLean.DHashMap
